logic/logic_lemmas.v
@@ -47,28 +47,34 @@ Qed.
 (* ==================== Substitution is Safe in Logic ==================== *)
 
 Fixpoint veq_subs_logicsafe_weak
-  Γ Γ' A v i v_s v_s' A_s (orig: has_vtype Γ' v A) {struct orig} :
-  veq A_s Γ v_s v_s' -> Γ' = ctx_insert Γ i A_s -> ctx_len Γ >= i ->
-  veq A Γ (v_subs v i v_s) (v_subs v i v_s')
+  Γ Γ' Ψ A v (orig: has_vtype Γ' v A) i v_s v_s' A_s {struct orig} :
+  judg Γ Ψ (Veq A_s v_s v_s') -> Γ' = ctx_insert Γ i A_s -> ctx_len Γ >= i ->
+  judg Γ Ψ (Veq A (v_subs v i v_s) (v_subs v i v_s'))
 
 with ceq_subs_logicsafe_weak
-  Γ Γ' C c i v_s v_s' A_s (orig: has_ctype Γ' c C) {struct orig} :
-  veq A_s Γ v_s v_s' -> Γ' = ctx_insert Γ i A_s -> ctx_len Γ >= i ->
-  ceq C Γ (c_subs c i v_s) (c_subs c i v_s')
+  Γ Γ' Ψ C c (orig: has_ctype Γ' c C) i v_s v_s' A_s {struct orig} :
+  judg Γ Ψ (Veq A_s v_s v_s') -> Γ' = ctx_insert Γ i A_s -> ctx_len Γ >= i ->
+  judg Γ Ψ (Ceq C (c_subs c i v_s) (c_subs c i v_s'))
 
 with heq_subs_logicsafe_weak
-  Γ Γ' Σ D h i v_s v_s' A_s (orig: has_htype Γ' h Σ D) {struct orig} :
-  veq A_s Γ v_s v_s' -> Γ' = ctx_insert Γ i A_s -> ctx_len Γ >= i ->
-  heq Σ D Γ (h_subs h i v_s) (h_subs h i v_s').
+  Γ Γ' Ψ Σ D h (orig: has_htype Γ' h Σ D) i v_s v_s' A_s {struct orig} :
+  judg Γ Ψ (Veq A_s v_s v_s') -> Γ' = ctx_insert Γ i A_s -> ctx_len Γ >= i ->
+  judg Γ Ψ (Heq Σ D (h_subs h i v_s) (h_subs h i v_s')).
 
 Proof.
 all: rename veq_subs_logicsafe_weak into VEQ.
 all: rename ceq_subs_logicsafe_weak into CEQ.
 all: rename heq_subs_logicsafe_weak into HEQ.
+all: intros vseq ctxs clen.
+all: assert (forall A, wf_vtype A -> 
+      judg (CtxU Γ A) (hyp_shift Ψ 1 0) 
+        (Veq A_s (v_shift v_s 1 0) (v_shift v_s' 1 0)) ) as vseq_ext by
+  (intros; eapply judg_shift_typesafe in vseq; simpl in vseq; eauto).
 {
-intros vseq ctxs clen. apply Veq; try (inv orig; eassumption).
-eapply v_subs_typesafe; inv vseq; eauto. 
-eapply v_subs_typesafe; inv vseq; eauto.
+apply WfJudg. apply WfVeq.
+{ inv vseq. inv H. eapply v_subs_typesafe; eauto. }
+{ inv vseq. inv H. eapply v_subs_typesafe; eauto. }
+{ inv vseq. auto. }
 destruct orig. destruct H1.
 + clear VEQ CEQ HEQ. unfold v_subs. simpl. apply VeqUnit.
 + clear VEQ CEQ HEQ. unfold v_subs. simpl. apply VeqInt.
@@ -77,17 +83,18 @@ destruct orig. destruct H1.
   - rewrite v_negshift_shift, v_negshift_shift, v_shift_0, v_shift_0.
     apply Nat.eqb_eq in ni. subst. rewrite get_ctx_insert_new in H1. inv H1. 
     inv vseq. assumption. all: omega || assumption.
-  - assert (veq A Γ 
+  - assert (judg Γ Ψ (Veq A 
       (if i <=? n then Var (n-1) else Var n)
-      (if i <=? n then Var (n-1) else Var n)).
+      (if i <=? n then Var (n-1) else Var n))).
     apply veq_refl. apply TypeV; auto.
-    { inv vseq. inv H2. assumption. }
+    { inv vseq. inv H2. inv H8. assumption. }
     destruct (i<=?n) eqn: cmp.
     * apply TypeVar. subst. erewrite get_ctx_insert_changed.
       all: apply Nat.eqb_neq in ni; apply leb_complete in cmp.
       assert (1+(n-1)=n) by omega. rewrite H2. eauto. omega.
     * apply TypeVar. subst. erewrite get_ctx_insert_unchanged. eauto.
       apply leb_complete_conv in cmp. assumption.
+    * inv vseq. auto.
     * inv H2. assumption.
 + clear CEQ HEQ. unfold v_subs. simpl. apply VeqPair; eapply VEQ; eauto.
 + clear CEQ HEQ. unfold v_subs. simpl. apply VeqInl. eapply VEQ; eauto.
@@ -95,21 +102,29 @@ destruct orig. destruct H1.
 + clear CEQ HEQ. unfold v_subs. simpl. apply VeqListNil.
 + clear CEQ HEQ. unfold v_subs. simpl. apply VeqListCons; eapply VEQ; eauto.
 + clear VEQ HEQ. unfold v_subs. unfold c_subs in CEQ. simpl. 
-  apply VeqFun. rewrite v_shift_comm, (v_shift_comm _ _ _ _ v_s'). 
-  eapply CEQ; eauto. apply veq_shift_typesafe; eauto.
+  apply VeqFun. rewrite v_shift_comm, (v_shift_comm _ _ _ _ v_s').
+  eapply CEQ; eauto. apply vseq_ext.
   inv H0. auto. subst. apply ctx_insert_extend. simpl. all: omega.
 + clear VEQ. unfold v_subs. unfold c_subs in CEQ. unfold h_subs in HEQ. simpl.
   eapply VeqHandler. 3: apply csubtype_refl; inv H0; assumption.
   - rewrite v_shift_comm, (v_shift_comm _ _ _ _ v_s'). eapply CEQ; eauto.
-    apply veq_shift_typesafe; eauto. inv H0. inv H6. assumption.
+    apply vseq_ext. inv H0. inv H6. assumption.
     subst. apply ctx_insert_extend. simpl. all: omega.
   - eapply HEQ; eauto.
-+ assert (veq A' Γ (v_subs v i v_s) (v_subs v i v_s')).
-  eapply veq_subtype; eauto. inv H3. assumption.
++ assert (judg Γ Ψ (Veq A' (v_subs v i v_s) (v_subs v i v_s'))).
+  eapply veq_subtype. 2: reflexivity. all: eauto. inv H3. assumption.
 }{
-intros vseq ctxs clen. apply Ceq; try (inv orig; eassumption).
-eapply c_subs_typesafe; inv vseq; eauto. 
-eapply c_subs_typesafe; inv vseq; eauto.
+assert (forall A B, wf_vtype A -> wf_vtype B -> 
+judg (CtxU (CtxU Γ B) A) (hyp_shift Ψ 2 0) 
+  (Veq A_s (v_shift v_s 2 0) (v_shift v_s' 2 0)) ) as vseq_extext.
+{ intros. eapply judg_shift_typesafe in vseq. 
+  eapply judg_shift_typesafe in vseq. 
+  rewrite hyp_shift_shift, form_shift_shift in vseq. simpl in vseq.
+  eauto. all: eauto. } 
+apply WfJudg. apply WfCeq.
+{ inv vseq. inv H. eapply c_subs_typesafe; eauto. }
+{ inv vseq. inv H. eapply c_subs_typesafe; eauto. }
+{ inv vseq. auto. }
 destruct orig. destruct H1.
 + clear CEQ HEQ. unfold c_subs. unfold v_subs in VEQ. simpl.
   apply CeqRet. eauto.
@@ -118,157 +133,72 @@ destruct orig. destruct H1.
 + clear HEQ. unfold c_subs in *. unfold v_subs in VEQ. simpl.
   eapply CeqΠMatch. eauto.
   rewrite v_shift_comm, (v_shift_comm _ _ _ _ v_s'). eapply CEQ; eauto.
-  rewrite <-(v_shift_shift 1 1), <-(v_shift_shift 1 1).
-  apply veq_shift_typesafe. apply veq_shift_typesafe. eauto.
+  apply vseq_extext.
   inv H1. inv H4. assumption. inv H1. inv H4. assumption.
   subst. rewrite ctx_insert_extend, ctx_insert_extend. reflexivity.
   simpl. all: omega.
 + clear HEQ. unfold c_subs in *. unfold v_subs in VEQ. simpl.
   eapply CeqΣMatch. eauto.
   all: rewrite v_shift_comm, (v_shift_comm _ _ _ _ v_s').
-  eapply CEQ; eauto. apply veq_shift_typesafe; eauto.
-  inv H1. inv H5. assumption. subst. apply ctx_insert_extend. simpl.
-  all: try omega. eapply CEQ; eauto. apply veq_shift_typesafe; eauto.
-  inv H1. inv H5. assumption. subst. apply ctx_insert_extend. simpl. omega.
+  eapply CEQ; eauto. apply vseq_ext. inv H1. inv H5.
+  assumption. subst. apply ctx_insert_extend. simpl.
+  all: try omega. 
+  eapply CEQ; eauto. apply vseq_ext. inv H1. inv H5.
+  assumption. subst. apply ctx_insert_extend. simpl. omega.
 + clear HEQ. unfold c_subs in *. unfold v_subs in VEQ. simpl.
   eapply CeqListMatch; eauto.
   rewrite v_shift_comm, (v_shift_comm _ _ _ _ v_s'). eapply CEQ; eauto.
-  rewrite <-(v_shift_shift 1 1), <-(v_shift_shift 1 1).
-  apply veq_shift_typesafe. apply veq_shift_typesafe. eauto.
-  inv H1. inv H5. assumption. inv H1. assumption.
+  apply vseq_extext. inv H1. assumption. inv H1. inv H5. assumption.
   subst. rewrite ctx_insert_extend, ctx_insert_extend. reflexivity.
   simpl. all: omega.
 + clear HEQ VEQ. unfold c_subs in *. simpl.
   eapply CeqDoBind. eauto. rewrite v_shift_comm, (v_shift_comm _ _ _ _ v_s').
-  eapply CEQ; eauto. apply veq_shift_typesafe; eauto.
+  eapply CEQ; eauto. apply vseq_ext.
   inv H1. inv H4. assumption. subst. apply ctx_insert_extend. simpl. all: omega.
 + clear HEQ. unfold c_subs. unfold v_subs in *. simpl. eapply CeqApp; eauto.
 + clear HEQ. unfold c_subs in *. unfold v_subs in *. simpl.
   eapply CeqHandle; eauto.
 + clear VEQ HEQ. unfold c_subs in *. simpl. eapply CeqLetRec.
   - rewrite v_shift_comm, (v_shift_comm _ _ _ _ v_s'). eapply CEQ; eauto.
-    rewrite <-(v_shift_shift 1 1), <-(v_shift_shift 1 1 _ v_s'). 
-    apply veq_shift_typesafe. apply veq_shift_typesafe. eauto.
-    inv H1. inv H3. inv H8. eauto. inv H1. inv H3. eauto.
+    apply vseq_extext.
+    inv H1. inv H3. eauto. inv H1. inv H3. inv H8. eauto.
     subst. rewrite ctx_insert_extend, ctx_insert_extend. reflexivity.
     simpl. all: omega.
   - rewrite v_shift_comm, (v_shift_comm _ _ _ _ v_s'). eapply CEQ; eauto.
-    apply veq_shift_typesafe. eauto. inv H2. inv H3. assumption.
+    apply vseq_ext. inv H2. inv H3. assumption.
     subst. apply ctx_insert_extend. simpl. all: omega.
 + clear HEQ. unfold c_subs in *. unfold v_subs in *. simpl. eapply CeqOp; eauto.
   rewrite v_shift_comm, (v_shift_comm _ _ _ _ v_s'). eapply CEQ; eauto.
-  apply veq_shift_typesafe. eauto. inv H3. inv H4. assumption.
+  apply vseq_ext. inv H3. inv H4. assumption.
   subst. apply ctx_insert_extend. simpl. all: omega.
-+ assert (ceq C' Γ (c_subs c i v_s) (c_subs c i v_s')).
-  eapply ceq_subtype; eauto. inv H3. assumption.
++ assert (judg Γ Ψ (Ceq C' (c_subs c i v_s) (c_subs c i v_s'))).
+  eapply ceq_subtype. 2: reflexivity. all: eauto. inv H3. assumption.
 }{
-intros vseq ctxs clen. destruct orig. destruct H2.
+(* Delaying the WfJudg allows us to use the heq_case_extend_structural. *)
+destruct orig. destruct H2.
 + clear VEQ CEQ HEQ. 
-  assert (has_htype Γ CasesØ SigØ D).
-  {apply TypeH. inv vseq. inv H2. 2:apply WfSigØ. all:auto. apply TypeCasesØ. }
-  eapply Heq; eauto; try (apply sig_subtype_refl; assumption). 
-  all: unfold h_subs; simpl. apply HeqSigØ.
+  unfold h_subs; simpl.
+  apply WfJudg. eapply WfHeq. auto.
+  all: apply HeqSigØ || apply TypeH || apply sig_subtype_refl || auto.
+  all: apply WfSigØ || apply TypeCasesØ || inv vseq; auto.
+  all: inv H2; inv H8; auto.
 + unfold h_subs in *. unfold c_subs in *. simpl.
   eapply HEQ in H3; eauto. eapply CEQ in H4. all: clear VEQ CEQ HEQ.
-  4: instantiate (2:=CtxU (CtxU Γ (TyFun Bop D)) Aop).
+  4: instantiate (2:=CtxU (CtxU Γ Aop) (TyFun Bop D)).
   Focus 3. 
     erewrite <-ctx_insert_extend. f_equal. erewrite <-ctx_insert_extend.
     f_equal. eauto.
   Focus 2.
-    eapply veq_shift_typesafe. eapply veq_shift_typesafe. eauto.
-    apply WfTyFun. all: inv H0; auto.
-  eapply heq_case_extend_structural; eauto.
+    eapply judg_shift_typesafe in vseq. eapply judg_shift_typesafe in vseq.
+    simpl in vseq. eauto. apply WfTyFun. all: inv H0; auto.
+  simpl in H4.
+  eapply heq_case_extend_structural; auto.
   all: try rewrite v_shift_shift, v_shift_shift in H4; simpl in *.
   - apply negshift_get_case_None. apply sub_get_case_None. assumption.
   - apply negshift_get_case_None. apply sub_get_case_None. assumption.
-  - rewrite v_shift_comm, (v_shift_comm _ _ _ _ v_s'). assumption. all: omega.
+  - rewrite v_shift_comm, (v_shift_comm _ _ _ _ v_s'). 
+    rewrite hyp_shift_shift in H4. assumption. all: omega.
   - omega.
 }
 Qed.
 
-
-Fixpoint veq_subs_logicsafe
-  Γ Γ' A v1 v2 i v_s v_s' A_s (orig: veq A Γ' v1 v2) {struct orig} :
-  veq A_s Γ v_s v_s' -> Γ' = ctx_insert Γ i A_s -> ctx_len Γ >= i ->
-  veq A Γ (v_subs v1 i v_s) (v_subs v2 i v_s')
-
-with ceq_subs_logicsafe
-  Γ Γ' C c1 c2 i v_s v_s' A_s (orig: ceq C Γ' c1 c2) {struct orig} :
-  veq A_s Γ v_s v_s' -> Γ' = ctx_insert Γ i A_s -> ctx_len Γ >= i ->
-  ceq C Γ (c_subs c1 i v_s) (c_subs c2 i v_s')
-
-with heq_subs_logicsafe
-  Γ Γ' Σ D h1 h2 i v_s v_s' A_s (orig: heq Σ D Γ' h1 h2) {struct orig} :
-  veq A_s Γ v_s v_s' -> Γ' = ctx_insert Γ i A_s -> ctx_len Γ >= i ->
-  heq Σ D Γ (h_subs h1 i v_s) (h_subs h2 i v_s').
-Proof.
-all: intros vseq ctxs clen.
-{
-assert (veq A Γ (v_subs v1 i v_s) (v_subs v1 i v_s')).
-eapply veq_subs_logicsafe_weak; eauto. inv orig. eauto.
-eapply veq_trans; eauto. eapply veq_subs_typesafe; eauto. inv vseq. auto.
-}{
-assert (ceq C Γ (c_subs c1 i v_s) (c_subs c1 i v_s')).
-eapply ceq_subs_logicsafe_weak; eauto. inv orig. eauto.
-eapply ceq_trans; eauto. eapply ceq_subs_typesafe; eauto. inv vseq. auto.
-}{
-inv orig.
-assert (heq Σ D Γ (h_subs h1 i v_s) (h_subs h1 i v_s')).
-eapply heq_subtype. 3:exact H0. eapply heq_subs_logicsafe_weak. all: eauto.
-eapply heq_trans; eauto. eapply heq_subs_typesafe; eauto.
-eapply Heq. 2: exact H0. all:eauto. inv vseq. assumption.
-}
-Qed.
-
-
-(* ==================== Context Modification ==================== *)
-
-Fixpoint veq_join_ctxs Γ Γ' v1 v2 A:
-  wf_ctx Γ' -> veq A Γ v1 v2 -> veq A (join_ctxs Γ' Γ) v1 v2
-with ceq_join_ctxs Γ Γ' c1 c2 C:
-  wf_ctx Γ' -> ceq C Γ c1 c2 -> ceq C (join_ctxs Γ' Γ) c1 c2
-with heq_join_ctxs Γ Γ' h1 h2 Σ D:
-  wf_ctx Γ' -> heq Σ D Γ h1 h2 -> heq Σ D (join_ctxs Γ' Γ) h1 h2 .
-Proof.
-all: intros wfc' orig.
-+ destruct Γ'.
-  - rewrite join_ctxs_CtxØ. auto.
-  - rewrite join_ctxs_CtxU. auto. 
-    apply veq_join_ctxs. inv wfc'. eauto.
-    rewrite <-(v_shift_too_high v1 1 (ctx_len Γ)).
-    rewrite <-(v_shift_too_high v2 1 (ctx_len Γ)).
-    apply veq_insert_typesafe. auto. inv wfc'. auto. 
-    all: eapply has_vtype_is_under_ctx; inv orig; eauto.
-+ destruct Γ'.
-  - rewrite join_ctxs_CtxØ. auto.
-  - rewrite join_ctxs_CtxU. auto. 
-    apply ceq_join_ctxs. inv wfc'. eauto.
-    rewrite <-(c_shift_too_high c1 1 (ctx_len Γ)).
-    rewrite <-(c_shift_too_high c2 1 (ctx_len Γ)).
-    apply ceq_insert_typesafe. auto. inv wfc'. auto. 
-    all: eapply has_ctype_is_under_ctx; inv orig; eauto.
-+ destruct Γ'.
-  - rewrite join_ctxs_CtxØ. auto.
-  - rewrite join_ctxs_CtxU. auto. 
-    apply heq_join_ctxs. inv wfc'. eauto.
-    rewrite <-(h_shift_too_high h1 1 (ctx_len Γ)).
-    rewrite <-(h_shift_too_high h2 1 (ctx_len Γ)).
-    apply heq_insert_typesafe. auto. inv wfc'. auto.
-    all: inv orig; eapply has_htype_is_under_ctx; eauto.
-Qed.
-
-(* 
-Lemma handle_t_makes_sense Γ' x c_r h A Σ E D Γ Z T:
-  has_vtype Γ' (Handler x c_r h)  (TyHandler (CTy A Σ E) D) ->
-  wf_t Γ Z T Σ ->
-  ceq D (join_ctxs Γ' (join_ctx_tctx Γ Z D))
-    (handle_t (ctx_len Γ) (tctx_len Z) h T)
-    (Handle 
-      (Sub.v_shift (Handler x c_r h) (ctx_len Γ + tctx_len Z) 0) 
-      (instantiate_t (tctx_len Z) T))
-.
-Proof.
-induction T; intros htys wft.
-+ simpl. *)
-
-(* h : C => D -> c1 ~C c2 -> with h handle c1 ~D with h handle c2 *)
